Add examples file

2016/Ext_Structures.thy
@@ -15,6 +15,7 @@ section{*Pair, Tuples and Records*
 text{* In this section,we extend our current lambda calculus with extended structures (pairs, tuples, records)*}
 
 datatype ltype =
+  Nat  |
   Bool |
   T (num:nat) |
   Unit |
@@ -32,6 +33,8 @@ datatype lterm =
   LFalse |
   LIf (bool_expr: lterm) (then_expr: lterm) (else_expr: lterm) |
   LVar nat |
+  LNat nat |
+  LPlus lterm lterm |
   LAbs (arg_type: ltype) (body: lterm) |
   LApp lterm lterm |
   unit |
@@ -50,7 +53,7 @@ datatype lterm =
   inl lterm ltype ("inl/ (_)/ as/ (_)" [100,100]200) |
   inr lterm ltype ("inr/ (_)/ as/ (_)" [100,100]200) |
   CaseSum lterm nat lterm nat lterm ("Case/ (_)/ of/ Inl/ (_)/ \<Rightarrow>/ (_)/ |/ Inr/ (_)/ \<Rightarrow>/ (_)" [100, 100,100, 100, 100]200) |
-  Variant string lterm ltype ("<(_):=(_)> as (_)" [100,100]200) |
+  Variant string lterm ltype ("<(_):=(_)> as (_)" [100,55] 200) |
   CaseVar lterm "string list" "nat list" "lterm list" ("Case/ (_)/ of/ <(_):=(_)>/ \<Rightarrow>/ (_)" [100,100,100,100]200) 
     
 
@@ -60,6 +63,8 @@ primrec shift_L :: "int \<Rightarrow> nat \<Rightarrow> lterm \<Rightarrow> lter
   "shift_L d c LFalse = LFalse" |
   "shift_L d c (LIf t1 t2 t3) = LIf (shift_L d c t1) (shift_L d c t2) (shift_L d c t3)" |
   "shift_L d c (LVar k) = LVar (if k < c then k else nat (int k + d))" |
+  "shift_L d c (LNat n) = LNat n"|
+  "shift_L d c (LPlus t1 t2) = LPlus (shift_L d c t1) (shift_L d c t2)"|
   "shift_L d c (LAbs T' t) = LAbs T' (shift_L d (Suc c) t)" |
   "shift_L d c (LApp t1 t2) = LApp (shift_L d c t1) (shift_L d c t2)" |
   "shift_L d c unit = unit" |
@@ -88,15 +93,13 @@ primrec shift_L :: "int \<Rightarrow> nat \<Rightarrow> lterm \<Rightarrow> lter
   "shift_L d c (Case t of <L:=I> \<Rightarrow> LT) = 
     (Case (shift_L d c t) of <L:= (map (\<lambda>x. if x\<ge> c then (nat (int x + d)) else x) I)> \<Rightarrow> map (shift_L d c) LT)"
 
-lemma map_to_rep[simp,cong,fundef_cong]:"\<And>i. i<length S \<Longrightarrow> j\<noteq>S!i \<Longrightarrow> map (\<lambda>x. if j=x then id else G) I = replicate (length S) G" sorry
-lemma apply_repl[simp,cong,fundef_cong]: "n>0 \<Longrightarrow> apply_L (replicate n G) TL = map G TL" sorry
-
-
 function subst_L :: "nat \<Rightarrow> lterm \<Rightarrow> lterm \<Rightarrow> lterm" where
   "subst_L j s LTrue = LTrue" |
   "subst_L j s LFalse = LFalse" |
   "subst_L j s (LIf t1 t2 t3) = LIf (subst_L j s t1) (subst_L j s t2) (subst_L j s t3)" |
   "subst_L j s (LVar k) = (if k = j then s else LVar k)" |
+  "subst_L j s (LNat n) = LNat n"|
+  "subst_L j s (LPlus t1 t2) = LPlus (subst_L j s t1) (subst_L j s t2)"|
   "subst_L j s (LAbs T' t) = LAbs T' (subst_L (Suc j) (shift_L 1 0 s) t)" |
   "subst_L j s (LApp t1 t2) = LApp (subst_L j s t1) (subst_L j s t2)" |
   "subst_L j s unit = unit" |
@@ -174,6 +177,7 @@ inductive is_value_L :: "lterm \<Rightarrow> bool" where
   VFalse: "is_value_L LFalse" |
   VAbs  :"is_value_L (LAbs T' t)" |
   VUnit :"is_value_L unit" |
+  VNat  : "is_value_L (LNat n)"|
   VPair :"is_value_L v1 \<Longrightarrow> is_value_L v2 \<Longrightarrow> is_value_L (\<lbrace>v1,v2\<rbrace>)" |
   VTuple:"(\<And>i.0\<le>i \<Longrightarrow> i<length L \<Longrightarrow> is_value_L (L!i)) \<Longrightarrow> is_value_L (Tuple L)" |
   VRCD  :"(\<And>i.0\<le>i \<Longrightarrow> i<length LT \<Longrightarrow> is_value_L (LT!i)) \<Longrightarrow> is_value_L (Record L LT)"|
@@ -185,6 +189,8 @@ primrec FV :: "lterm \<Rightarrow> nat set" where
   "FV LFalse = {}" |
   "FV (LIf t1 t2 t3) = FV t1 \<union> FV t2 \<union> FV t3" |
   "FV (LVar x) = {x}" |
+  "FV (LNat n) = {}"|
+  "FV (LPlus t1 t2) = FV t1 \<union> FV t2"|
   "FV (LAbs T1 t) = image (\<lambda>x. x - 1) (FV t - {0})" |
   "FV (LApp t1 t2) = FV t1 \<union> FV t2" |
   "FV unit = {}" |
@@ -235,6 +241,7 @@ fun fill::"(nat \<Rightarrow> lterm) \<Rightarrow> lterm \<Rightarrow> lterm" wh
 "fill \<Delta> (LIf c t1 t2)               = LIf (fill \<Delta> c) (fill \<Delta> t1) (fill \<Delta> t2)" |
 "fill \<Delta> (LAbs A t1)                 = LAbs A (fill \<Delta> t1)" |
 "fill \<Delta> (LApp t1 t2)                = LApp (fill \<Delta> t1) (fill \<Delta> t2)" |
+"fill \<Delta> (LPlus t1 t2)                = LPlus (fill \<Delta> t1) (fill \<Delta> t2)" |
 "fill \<Delta> (Seq t1 t2)                 =  Seq (fill \<Delta> t1) (fill \<Delta> t2)" |
 "fill \<Delta> (t1 as A)                   = (fill \<Delta> t1) as A" |
 "fill \<Delta> (Let var x := t1 in t2)     = (Let var x := (fill \<Delta> t1) in (fill \<Delta> t2))" |
@@ -281,7 +288,11 @@ inductive eval1_L :: "lterm \<Rightarrow> lterm \<Rightarrow> bool" where
   eval1_LApp_LAbs:
     "is_value_L v2 \<Longrightarrow> eval1_L (LApp (LAbs T' t12) v2)
       (shift_L (-1) 0 (subst_L 0 (shift_L 1 0 v2) t12))" |
-  
+
+  -- "Rules relating to the evaluation of Plus"
+  eval1_LPlus:
+    "eval1_L (LPlus (LNat n1) (LNat n2)) (LNat (n1+n2))"|
+
  -- "Rules relating to evaluation of sequence"
   
   eval1_L_Seq:
@@ -377,6 +388,10 @@ inductive has_type_L :: "lcontext \<Rightarrow> lterm \<Rightarrow> pcontext \<R
   -- \<open>Rules relating to the type of the constructs of the $\lambda$-calculus\<close>
   has_type_LVar:
     "(x, T') |\<in>| \<Gamma> \<Longrightarrow> \<Gamma> \<turnstile> \<lparr>LVar x|;|fill \<delta>\<rparr> |:| (T')" |
+  have_type_LNat:
+    "\<Gamma> \<turnstile> \<lparr>LNat n|;| fill \<delta>\<rparr> |:| Nat"|
+  have_type_LPlus:
+    "\<Gamma> \<turnstile> \<lparr>t1|;| fill \<delta>\<rparr> |:| Nat \<Longrightarrow> \<Gamma> \<turnstile> \<lparr>t2|;| fill \<delta>\<rparr> |:| Nat \<Longrightarrow> \<Gamma> \<turnstile> \<lparr>LPlus t1 t2|;| fill \<delta>\<rparr> |:| Nat" |  
   has_type_LAbs:
     "(\<Gamma> |,| T1) \<turnstile> \<lparr>t2|;| fill (shift_L 1 (Suc (nbinder t2)) \<circ> \<delta>)\<rparr> |:| T2 \<Longrightarrow> \<Gamma> \<turnstile> \<lparr>LAbs T1 t2|;|fill \<delta>\<rparr> |:| (T1 \<rightarrow> T2)" |
   has_type_LApp:
@@ -647,14 +662,14 @@ next
   case (has_type_ProjT i TL \<Gamma>1 t \<delta>1)
     show ?case
       using has_type_ProjT(4)[OF has_type_ProjT(5,6)]
-            "has_type_L.intros"(15)[OF has_type_ProjT(1,2)]
+            "has_type_L.intros"(17)[OF has_type_ProjT(1,2)]
       by fastforce
 next
   case (has_type_RCD L LT TL \<Gamma> \<delta>1)
     show ?case
       using has_type_RCD(1-4) nth_map[of _ LT "shift_L 1 n"]
             has_type_RCD(6)[OF _ has_type_RCD(7,8)]           
-      by (force intro!: "has_type_L.intros"(16))+
+      by (force intro!: "has_type_L.intros"(18))+
 next
   case (has_type_Let \<Gamma>1 t1 \<delta>1 A x t2 B)
     have 1:"n\<le>x \<Longrightarrow> ?case"
@@ -662,14 +677,14 @@ next
         assume le_x: "n\<le>x"
         show ?case
           using has_type_Let(4-6) le_x
-                "has_type_L.intros"(10)[OF has_type_Let(2)[OF has_type_Let(5,6)], of "Suc x"]
+                "has_type_L.intros"(12)[OF has_type_Let(2)[OF has_type_Let(5,6)], of "Suc x"]
           by  (simp add: le_x del: Fun.comp_apply,
                 metis insert_nth_take_drop rep_ins replace_inv_length append_Cons append_Nil2 append_eq_append_conv_if)
       qed
 
     have "n>x \<Longrightarrow> ?case"
       using has_type_Let(4-6) rep_ins2[OF _ has_type_Let(6), of x S A]
-            "has_type_L.intros"(10)[OF has_type_Let(2)[OF has_type_Let(5,6)], of x]
+            "has_type_L.intros"(12)[OF has_type_Let(2)[OF has_type_Let(5,6)], of x]
       by (simp del: Fun.comp_apply,
             metis append_Cons append_Nil insert_nth_take_drop replace_inv_length)
     with 1 show ?case 
@@ -682,7 +697,7 @@ next
         fix x
         show "(shift_L 1 n \<circ> (\<lambda>x. <|V x|>)) x = (\<lambda>x. <|V x|>) x" 
           using Fun.comp_apply[of "shift_L 1 n" "\<lambda>x. <|V x|>" x]
-                "shift_L.simps"(18)
+                "shift_L.simps"(20)
           by metis
       qed
     have 1:"insert_nth n S \<Gamma>1 \<turnstile> \<lparr>(fill (shift_L 1 n \<circ> \<delta>) ^^ m) (<|V k|>)|;|id\<rparr> |:| A" 
@@ -692,7 +707,7 @@ next
     have "set (patterns ((fill (shift_L 1 n \<circ> \<delta>) ^^ m) (<|V k|>))) = {}"
       using has_type_PatternVar(3,4) pattern_fill_shift[of m 1 n \<delta> "<|V k|>"]
       by fastforce  
-    with 1 show ?case by (auto intro:"has_type_L.intros"(18)[where \<delta>="(shift_L 1 n \<circ> \<delta>)"])
+    with 1 show ?case by (auto intro:"has_type_L.intros"(20)[where \<delta>="(shift_L 1 n \<circ> \<delta>)"])
 next
   case (has_type_LetPattern p t1 \<delta>1 \<Gamma>1 \<delta>2 B t2 A)
     have 1:"Lmatch p (shift_L 1 n t1) (shift_L 1 n \<circ> \<delta>1)"
@@ -747,7 +762,7 @@ next
              replace_inv_length not_le
       by metis+
     show ?case
-      by (auto)(insert A B1 B2 B3 B4 "has_type_L.intros"(23), force+)
+      by (auto)(insert A B1 B2 B3 B4 "has_type_L.intros"(25), force+)
 next
   case (has_type_CaseV L I TL LT \<Gamma> t \<delta>1 A)
     have branches_wtyped:"\<forall>i<length L.
@@ -800,7 +815,7 @@ next
     show ?case
       using has_type_CaseV(1-4) has_type_CaseV(6)[OF has_type_CaseV(8,9)]
             branches_wtyped
-      by (force intro!: "has_type_L.intros"(25))+      
+      by (force intro!: "has_type_L.intros"(27))+      
 qed (auto intro!: has_type_L.intros simp: nth_append min_def)
 
 lemma fill_keep_value:
