2016/Variant_Type_examples.thy
@@ -1,0 +1,30 @@
+theory Variant_Type_examples
+imports Main
+        Ext_Structures
+begin
+  
+abbreviation OptionType::"ltype \<Rightarrow> ltype" ("(_)/ option" [201]200) where
+"A option \<equiv> <[''none'',''some'']|,|[Unit,A]>"    
+ 
+abbreviation Table ::"ltype" where
+"Table \<equiv> Nat\<rightarrow>(Nat option)"
+
+abbreviation emptyTable ::"lterm" where
+"emptyTable \<equiv> LAbs Nat (<''none'':=unit> as Nat option)"  
+
+
+lemma "\<emptyset> \<turnstile> \<lparr>emptyTable |;| id\<rparr> |:| Table"
+ proof -
+   let ?inner_term = "<''none'':= unit> as (Nat option)"
+   have H:"[Nat] \<turnstile> \<lparr> ?inner_term|;| fill (shift_L 1 (Suc (nbinder ?inner_term))\<circ>(\<lambda>x. <|V x|>))\<rparr> |:| Nat option"
+     using has_type_Variant[of "[Nat]" unit "shift_L 1 (Suc (nbinder ?inner_term))\<circ>(\<lambda>x. <|V x|>)" "[Unit, Nat]" 0 "[''none'',''some'']"]
+           has_type_LUnit[of "[Nat]" "shift_L 1 (Suc (nbinder ?inner_term))\<circ>(\<lambda>x. <|V x|>)"] fill_id
+     by fastforce
+   
+   then show ?thesis     
+     using has_type_LAbs[of Nat \<emptyset> ?inner_term "\<lambda>x. <|V x|>" "Nat option"]
+           fill_id     
+     by auto
+qed
+      
+end
